ntt_chunk_base_case

crypto_examples/ntt.dfy
@@ -1,33 +1,35 @@
-include "pow2.dfy"
-include "omega.dfy"
 include "ntt_rec.dfy"
+include "index.dfy"
 
 module ntt {
     import opened Seq
     import opened Power
+    import opened Power2
     import opened DivMod
     import opened Mul
+
     import opened pows_of_2
     import opened omegas
     import opened ntt_rec
+    import opened rindex
 
     function A(): seq<elem>
         ensures |A()| == N == pow2(L).full;
 
     function Ar(): seq<elem>
         ensures |Ar()| == N == pow2(L).full;
-        // ensures forall i | 0 <= i < N :: Ar()[i] == 
+        ensures forall i | 0 <= i < N ::
+            Ar()[i] == A()[build_rev_index(i).v];
 
     lemma index_bounded_lemma(
         j: nat, k: nat, ki: nat,
-        m: pow2_t, step_count: pow2_t)
+        m: pow2_t)
         requires m.full >= 2;
         requires 0 <= j < m.full / 2;
         requires N == pow2(L).full;
         requires 1 <= m.exp <= L;
-        requires step_count == pow2_div(pow2(L), m);
         requires k == ki * m.full;
-        requires ki < step_count.full;
+        requires ki < pow2_div(pow2(L), m).full;
         ensures k + j + m.full / 2 < N;
     {
         pow2_basics(m);
@@ -43,73 +45,90 @@ module ntt {
             ki * m.full + m.full;
         == { LemmaMulIsDistributiveAddOtherWay(m.full, ki, 1); }
             (ki + 1) * m.full;
-        <= { assert ki + 1 <= step_count.full; LemmaMulInequalityAuto(); }
-            step_count.full * m.full;
+        <= { assert ki + 1 <= pow2_div(pow2(L), m).full; LemmaMulInequalityAuto(); }
+            pow2_div(pow2(L), m).full * m.full;
         ==
             N;
         }
     }
 
-    // lemma ntt_chunk_base_case(a': seq<elem>, 
-    //     k: nat, ki: nat, t: elem, u: elem,
-    //     m: pow2_t, step_count: pow2_t)
+    lemma ntt_chunk_base_case(a': seq<elem>, 
+        k: nat, ki: nat, t: elem, u: elem,
+        m: pow2_t)
 
-    //     requires |a'| == N == pow2(L).full;
-    //     requires m.exp == 1;
-    //     // requires step_count == pow2_div(pow2(L), m);
-    //     // requires k == ki * m.full;
-    //     // requires ki < step_count.full;
-    //     requires k < k + 1 < N;
-    
-    //     requires t == modmul(1, Ar()[k + 1]);
-    //     requires u == Ar()[k];
-    //     requires a'[k] == modadd(u, t);
-    //     requires a'[k+1] == modsub(u, t);
-    //     // ensures 
-    // {
-    //     calc == {
-    //         t;
-    //         modmul(1, Ar()[k + 1]);
-    //         (Ar()[k + 1]) % Q;
-    //         {
-    //             assume false;
-    //         }
-    //         Ar()[k + 1];
-    //     }
-
-    //     var len := pow2(0);
-    //     pow2_basics(len);
-
-    //     var even := Ar()[k..k+1];
-    //     var odd := Ar()[k+1..k+2];
-
-    //     ntt_rec_base_case(odd, len);
-    //     ntt_rec_base_case(even, len);
-
-    //     assert t == poly_eval(odd, omega_nk(len, 0));
-    //     assert u == poly_eval(even, omega_nk(len, 0));
-
-    //     var omg := omega_nk(len, 0);
-
-    //     y_k_value(even + odd, even, odd, pow2(0), pow2(1),
-    //             omg, k,
-    //             y_e_k: elem, y_o_k: elem, y_k: elem)
-    // }
-
-    method ntt_chunk_loop(a: seq<elem>,
-        k: nat, ki: nat,
-        m: pow2_t, step_count: pow2_t)
-    returns (a': seq<elem>)
-        // combine two chunks into one
-        requires |a| == N == pow2(L).full;
-        requires 1 <= m.exp <= L;
-        requires step_count == pow2_div(pow2(L), m);
+        requires |a'| == N == pow2(L).full;
+        requires m.exp == 1;
+        requires ki < pow2_div(pow2(L), m).full;
         requires k == ki * m.full;
-        requires ki < step_count.full;
+        requires k < k + 1 < N;
+
+        requires t == modmul(1, Ar()[k + 1]);
+        requires u == Ar()[k];
+        requires a'[k] == modadd(u, t);
+        requires a'[k+1] == modsub(u, t);
+
+        ensures a'[k] == poly_eval([Ar()[k], Ar()[k+1]], omega_nk(m, 0));
+        ensures a'[k+1] == poly_eval([Ar()[k], Ar()[k+1]], omega_nk(m, 1));
+    {
+        // nth_root_lemma();
+        pow2_basics(m);
+        var m' := pow2_half(m);
+
+        assert t == Ar()[k + 1] by {
+            assert Ar()[k + 1] < Q;
+        }
+
+        var even := Ar()[k..k+1];
+        var odd := Ar()[k+1..k+2];
+        var chunk := [Ar()[k], Ar()[k+1]];
+        assert chunk == even + odd;
+
+        assert Ar()[k] == A()[build_rev_index(k).v];
+        assert Ar()[k+1] == A()[build_rev_index(k+1).v];
+
+        var original := orignal_index(ki, 0, m);
+        assert original.v == k;
+
+        ntt_rec_base_case(odd, m');
+        ntt_rec_base_case(even, m');
+
+        assert u == poly_eval(even, omega_nk(m', 0));
+        assert t == poly_eval(odd, omega_nk(m', 0));
+
+        var omg := omega_nk(m, 0);
+
+        calc == {
+            modmul(omg, t);
+            {
+                LemmaPow0(omega_n(m));
+            }
+            modmul(1, t);
+        }
+
+        y_k_value(chunk, even, odd, pow2(0), pow2(1),
+            omg, 0, u, t, a'[k]);
+
+        y_k'_value(chunk, even, odd, pow2(0), pow2(1),
+            omg, 0, u, t, a'[k+1]);
+    }
+
+    method ntt_chunk_loop(a: seq<elem>, k: nat, ki: nat, m: pow2_t)
+    returns (a': seq<elem>)
+        // this loop works on a chunk of size m.full
+        // by combining two smaller chunks of size m.full/2
+        // m.full: the chunk size at the current level
+        requires |a| == N == pow2(L).full;
+        // m.exp: the level, go from 1 to L (log N)
+        requires 1 <= m.exp <= L;
+        // ki: the chunk id at current level, go from 0 to N/m
+        requires ki < pow2_div(pow2(L), m).full;
+        // k is ki times chunk size, points to start of the chunk
+        requires k == ki * m.full;
+
         requires m.exp == 1 ==> a == Ar();
     {
         a' := a;
-        var half_step := m.full / 2;
+        var len' := pow2_half(m);
         var omgm := omega_n(m);
 
         var omg := 1;
@@ -121,49 +140,34 @@ module ntt {
 
         pow2_basics(m);
 
-        index_bounded_lemma(0, k, ki, m, step_count);
+        index_bounded_lemma(0, k, ki, m);
 
-        while (j < half_step)
-            invariant 0 <= j <= half_step;
+        while (j < len'.full)
+            invariant 0 <= j <= len'.full;
             invariant omg == modpow(omgm, j);
             invariant |a'| == |a|;
-            invariant k + j + half_step <= N;
+            invariant k + j + len'.full <= N;
             invariant a[..k] == a'[..k];
-            invariant a[k+j..k+half_step] == a'[k+j..k+half_step];
-            invariant a[k+half_step+j..] == a'[k+half_step+j..];
-
+            invariant a[k+j..k+len'.full] == a'[k+j..k+len'.full];
+            invariant a[k+len'.full+j..] == a'[k+len'.full+j..];
         {
-            index_bounded_lemma(j, k, ki, m, step_count);
-            var t := modmul(omg, a[k + j + half_step]);
+            index_bounded_lemma(j, k, ki, m);
+            var t := modmul(omg, a[k + j + len'.full]);
             var u := a[k + j];
             a' := a'[k + j := modadd(u, t)];
-            a' := a'[k + j + half_step := modsub(u, t)];
+            a' := a'[k + j + len'.full := modsub(u, t)];
+
+           if m.exp == 1 {
+                ntt_chunk_base_case(a', k, ki, t, u, m);
+            }
 
             omg_inv(omgm, omg, m, j);
             omg := modmul(omg, omgm);
-
-            // if half_step == 1 {
-            //     ntt_chunk_base_case(a', k, ki, t, u, m, step_count);
-            // }
-
             j := j + 1;
         }
 
         assert a[..k] == a'[..k];
         assert a[k+m.full..] == a'[k+m.full..];
-
-        if m.exp == 1 {
-            assert half_step == 1;
-            // j := 0;
-            // index_bounded_lemma(j, s, k, ki, m, step_count);
-
-            // var t := modmul(omg, a[k + j + half_step]);
-            // var u := a[k + j];
-
-            // assert half_step == 1;
-            // assert a'[k + j] == modadd(u, t);
-
-        }
     }
 
     // method ntt_level_loop(a: seq<elem>, s: nat)
@@ -179,29 +183,26 @@ module ntt {
     //     assert omega_nk(m, 1) == omega_n(m) by {
     //         LemmaPow1Auto();
     //     }
-    //     var step_size := m.full;
 
-    //     var step_count := pow2_div(pow2(L), m);
-    //     // assert step_count.exp == L - m.exp;
-    
     //     var k := 0;
     //     var ki := 0;
 
-    //     while (ki < step_count.full) // at level s, each chunck is 2 ** s big
+    //     while (ki < pow2_div(pow2(L), m).full) 
+    //         // at level s, each chunck is 2 ** s big
     //         // invariant step_count == pow2_div(pow2(L), m);
     //         // invariant step_count.exp == L - m.exp;
-    //         invariant 0 <= k == ki * step_size;
+    //         invariant 0 <= k == ki * m.full;
     //     {
-    //         var k' := k + step_size;
+    //         var k' := k + m.full;
     //         var ki' := ki + 1;
 
-    //         var _ := ntt_chunk_loop(a, k, ki, m, step_count);
+    //         var _ := ntt_chunk_loop(a, k, ki, m);
 
-    //         assert k' == (ki + 1) * step_size by {
-    //             LemmaMulIsDistributiveAddOtherWay(step_size, ki, 1);
-    //             assert (ki + 1) * step_size == ki * step_size + 1 * step_size;
+    //         assert k' == (ki + 1) * m.full by {
+    //             LemmaMulIsDistributiveAddOtherWay(m.full, ki, 1);
+    //             assert (ki + 1) * m.full == ki * m.full + 1 * m.full;
     //         }
-    //         assert (ki + 1) * step_size > 0 by {
+    //         assert (ki + 1) * m.full > 0 by {
     //             LemmaMulStrictlyPositiveAuto();
     //         }
     //         k, ki := k', ki';
